io/TC.Monitorable.Hist.fst
@@ -31,8 +31,7 @@ class monitorable_hist
   (pre : t1 -> trace -> Type0)
   (post : t1 -> trace -> resexn t2 -> trace -> Type0)
   (pi : monitorable_prop) = {
-    (** this condition makes sure that all trace properties enforced by post are instrumented by pi **)
-    c1post : squash (forall x h lt. pre x h /\ enforced_locally pi h lt ==> (exists r. post x h r lt));
+    post_implies_pi : squash (forall x h lt r. pre x h /\ post x h r lt ==> enforced_locally pi h lt);
 }
 
 class checkable_hist_post
@@ -41,9 +40,12 @@ class checkable_hist_post
   (pre : t1 -> trace -> Type0)
   (post : t1 -> trace -> resexn t2 -> trace -> Type0)
   (pi : monitorable_prop) = {
-    cmonitorable: monitorable_hist #t1 #t2 pre post pi;
     (** the refinement makes sure that the post can not reject the halting of the execution by the insturmentation **)
     result_check : t1 -> trace -> r:resexn t2 -> trace -> (b:bool{r == Inr Contract_failure ==> b});
+    (** we want to make sure that result_check does not check any trace property, only properties related between
+        the result and the trace **)
+    (** this condition makes sure that all trace properties enforced by post are instrumented by pi **)
+    c1post : squash (forall x h lt. pre x h /\ enforced_locally pi h lt ==> (exists r. post x h r lt));
     (** this one makes sure that the post at the end is enough **)
     c2post: squash (forall x h r lt. pre x h /\ enforced_locally pi h lt /\ result_check x h r lt ==> post x h r lt);
 }
